code/Kody/IR.v
@@ -1,0 +1,4 @@
+Inductive IR (D : Type) : Type :=
+    | iota  : D -> IR D
+    | sigma : forall A : Type, (A -> IR D) -> IR D
+    | delta : forall A : Type, ((A -> D) -> IR D) -> IR D.
