code/Koło/InsertionSort.v
@@ -1,0 +1,79 @@
+Print list.
+
+Require Import List.
+Import ListNotations.
+
+Fixpoint ins
+  {A : Type} (cmp : A -> A -> bool) (x : A) (l : list A) : list A :=
+match l with
+    | [] => [x]
+    | h :: t =>
+        if cmp x h then x :: h :: t else h :: ins cmp x t
+end.
+
+Fixpoint insertionSort
+  {A : Type} (cmp : A -> A -> bool) (l : list A) : list A :=
+match l with
+    | [] => []
+    | h :: t => ins cmp h (insertionSort cmp t)
+end.
+
+Require Import Arith.
+
+Check leb.
+
+Compute leb 1 1.
+
+Compute insertionSort leb [6; 3; 4; 7; 1; 9].
+
+Inductive sorted {A : Type} (cmp : A -> A -> bool) : list A -> Prop :=
+    | sorted_nil : sorted cmp []
+    | sorted_singl : forall x : A, sorted cmp [x]
+    | sorted_cons :
+        forall (x y : A) (t : list A),
+          sorted cmp (y :: t) -> cmp x y = true ->
+            sorted cmp (x :: y :: t).
+
+Lemma example_sorted :
+  sorted leb [1; 3; 4; 6; 7; 9].
+Proof.
+  apply sorted_cons.
+    Focus 2. cbn. reflexivity.
+  apply sorted_cons.
+    Focus 2. cbn. reflexivity.
+  apply sorted_cons.
+    Focus 2. cbn. reflexivity.
+  apply sorted_cons.
+    Focus 2. cbn. reflexivity.
+  apply sorted_cons.
+    Focus 2. cbn. reflexivity.
+  apply sorted_singl.
+Qed.
+
+Lemma example_sorted' :
+  sorted leb [6; 3; 4; 7; 1; 9].
+Proof.
+  apply sorted_cons.
+    Focus 2. cbn.
+Abort.
+
+Lemma ins_sorted :
+  forall {A : Type} (cmp : A -> A -> bool) (x : A) (l : list A),
+    sorted cmp l -> sorted cmp (ins cmp x l).
+Proof.
+  induction l.
+    cbn. intros _. apply sorted_singl.
+    intro H. cbn. case_eq (cmp x a); intro.
+      apply sorted_cons.
+        assumption.
+        assumption.
+Admitted.
+
+Lemma insertionSort_sorted :
+  forall {A : Type} (cmp : A -> A -> bool) (l : list A),
+    sorted cmp (insertionSort cmp l).
+Proof.
+  induction l.
+    cbn. apply sorted_nil.
+    cbn. apply ins_sorted. assumption.
+Qed.
