code/Koło/NegatywnyProdukt.v
@@ -1,0 +1,27 @@
+CoInductive product (A : Type) (B : Type) : Type :=
+{
+    fst : A;
+    snd : B;
+}.
+
+Definition swap {A B : Type} (p : product A B) : product B A :=
+{|
+    fst := snd A B p;
+    snd := fst A B p;
+|}.
+
+Definition para_liczb : product nat nat :=
+{|
+    fst := 42;
+    snd := 1;
+|}.
+
+Compute fst nat nat para_liczb.
+Compute snd nat nat para_liczb.
+
+Lemma eq_product :
+  forall {A B : Type} (p q : product A B),
+    fst A B p = fst A B q -> snd A B p = snd A B q -> p = q.
+Proof.
+  destruct p, q. cbn. intros -> ->. reflexivity.
+Qed.
