code/Logika/coto.v
@@ -1,0 +1,10 @@
+Goal
+  ~
+  (forall (A : Type) (P : A -> Prop) (Q : Prop),
+    (forall x : A, P x -> Q) -> (forall x : A, P x) -> Q).
+Proof.
+  intro H.
+  apply (H False (fun _ => False)).
+    intros. assumption.
+    trivial.
+Qed.
